[statelib crdt] refactoring of params.

aneris/examples/crdt/statelib/user_model/params.v
@@ -4,24 +4,26 @@ From aneris.examples.crdt.spec Require Import crdt_spec.
 From aneris.examples.crdt.statelib.proof Require Import events.
 From aneris.examples.crdt.statelib.STS Require Import lst.
 From aneris.examples.crdt.statelib.user_model
-  Require Import model semi_join_lattices.
+     Require Import model semi_join_lattices.
+From stdpp Require Import gmap.
+From aneris.examples.crdt.spec Require Import crdt_base crdt_denot crdt_events crdt_time.
+From aneris.examples.crdt.statelib.proof Require Import events.
+From aneris.examples.crdt.statelib.user_model Require Import semi_join_lattices.
+From aneris.examples.crdt.statelib.STS Require Import lst.
 
-Section Params.
-  Context `{LogOp: Type, LogSt: Type,
-            !anerisG Mdl Σ,
-            !EqDecision LogOp, !Countable LogOp, !Lattice LogSt,
-            !CRDT_Params }.
+Section CohParams.
+  Context {LogOp : Type} {LogSt: Type}.
+  Context `{!EqDecision LogOp, !Countable LogOp}.
+  Context `{!CRDT_Params}.
+  Context `{!anerisG Mdl Σ}.
+
 
   (* User-supplied parameters when using the library. *)
-  Class StLib_Params := {
-    (* Serialization of operations. *)
-    StLib_StSerialization : serialization;
+  Class StLib_Coh_Params := {
+      (* Serialization of operations. *)
+      StLib_StSerialization : serialization;
 
-    (* CRDT model *)
-    StLib_Denot :> CrdtDenot LogOp LogSt;
-    StLib_Model :> StateCrdtModel LogOp LogSt;
-
-    (* Coherence between logical and physical state: for
+      (* Coherence between logical and physical state: for
        states, operations, and events (event = operation + timestamp).
 
        For example, for a counter CRDT the logical state is
@@ -29,18 +31,36 @@ Section Params.
        AnerisLang `val` (containing the integer).
        The correspondence is trivial in that case, but can
        be more complicated for other CRDTs. *)
-    StLib_Op_Coh : LogOp -> val -> Prop;
-    StLib_Op_Coh_Inj o1 o2 v : StLib_Op_Coh o1 v -> StLib_Op_Coh o2 v -> o1 = o2;
-    StLib_St_Coh : LogSt -> val -> Prop;
-    StLib_St_Coh_Inj o1 o2 v : StLib_St_Coh o1 v -> StLib_St_Coh o2 v -> o1 = o2;
-    StLib_StCoh_Ser st v : StLib_St_Coh st v -> Serializable StLib_StSerialization v;
-  }.
+      StLib_Op_Coh : LogOp -> val -> Prop;
+      StLib_Op_Coh_Inj o1 o2 v : StLib_Op_Coh o1 v -> StLib_Op_Coh o2 v -> o1 = o2;
+      StLib_St_Coh : LogSt -> val -> Prop;
+      StLib_St_Coh_Inj o1 o2 v : StLib_St_Coh o1 v -> StLib_St_Coh o2 v -> o1 = o2;
+      StLib_StCoh_Ser st v : StLib_St_Coh st v -> Serializable StLib_StSerialization v;
+    }.
+
+End CohParams.
+
+Section Params.
+  Context `{LogOp : Type, LogSt: Type}.
+  Context `{!EqDecision LogOp, !Countable LogOp}.
+  Context `{!CrdtDenot LogOp LogSt}.
+  Context `{!Lattice LogSt}.
+  Context `{!anerisG Mdl Σ}.
+  Context `{!CRDT_Params}.
+
+  (* User-supplied parameters when using the library. *)
+  Class StLib_Params := {
+      (* CRDT model *)
+      StLib_Denot :> CrdtDenot LogOp LogSt;
+      StLib_Model :> StateCrdtModel LogOp LogSt;
+      StLib_CohParams :> @StLib_Coh_Params LogOp LogSt;
+    }.
 
   Class StLib_Res `{!CRDT_Params} := {
-    StLib_CRDT_Res :> CRDT_Res_Mixin Mdl Σ LogOp;
-    StLib_InitToken : (fin (length CRDT_Addresses)) -> iProp Σ;
-    StLib_SocketProto : socket_interp Σ;
-  }.
+      StLib_CRDT_Res :> CRDT_Res_Mixin Mdl Σ LogOp;
+      StLib_InitToken : (fin (length CRDT_Addresses)) -> iProp Σ;
+      StLib_SocketProto : socket_interp Σ;
+    }.
 
 End Params.
 
