aneris/examples/crdt/statelib/examples/map_comb/statelib_map_comb_proof.v
@@ -27,20 +27,73 @@ Lemma map_dom_Some {E E'} `{!EqDecision E, !Countable E} (m: gmap E E') u v:
   m !! u = Some v → u ∈ gset_dom m.
 Proof. by intros?%elem_of_dom_2. Qed.
 
-Section Bloup.
 
-  Context `{latA: Lattice LogSt, !EqDecision LogOp, !Countable LogOp,
-            !@CrdtDenot LogOp LogSt timestamp_time _ _, !CRDT_Params,
-            inj_st: Inject LogSt val}.
-  Context {p: StLib_Params LogOp LogSt}.
+Section map_crdt_denot.
+  Context (LogOp : Type) (LogSt : Type).
+  Context `{!Log_Time}.
+  Context `{!EqDecision LogOp} `{!Countable LogOp}.
+  Context `{crdt_denotA : !CrdtDenot LogOp LogSt}.
+  Context `{!CRDT_Params}.
 
   Definition mapSt: Type := gmap string LogSt.
   Definition mapOp: Type := string * LogOp.
 
+  Global Instance map_op_eqdec: EqDecision mapOp.
+  Proof. apply prod_eq_dec. Defined.
+
+  Global Instance map_op_countable: Countable mapOp.
+  Proof. apply prod_countable. Qed.
+
+
+  Definition map_denot_def
+    (s: gset (Event mapOp)) (st: mapSt) : Prop :=
+    gset_dom st = gset_map (λ ev: Event mapOp, ev.(EV_Op).1) s
+    ∧ ∀ (str: string) (v: LogSt), st !! str = Some v →
+      crdt_denot (
+        gset_map
+          (λ e, {|EV_Op := e.(EV_Op).2;
+                  EV_Orig := e.(EV_Orig);
+                  EV_Time := e.(EV_Time) |})
+        (filter (λ ev, ev.(EV_Op).1 = str) s)) v.
+
+  Global Instance map_denot_fun : Rel2__Fun map_denot_def.
+  Proof.
+    constructor. intros s m m' [Hdom Helts][Hdom' Helts'].
+    apply map_eq. intros u.
+    destruct (m !! u)as[v|]eqn:Hms; destruct (m' !! u)as[v'|]eqn:Hm's.
+    - pose proof (Helts u v Hms) as A. pose proof (Helts' u v' Hm's) as B.
+      destruct (crdt_denotA.(crdt_denot_fun))as [Hden].
+      by rewrite Hms Hm's (Hden
+        (gset_map
+        (λ e : Event mapOp,
+           {|
+             EV_Op := (EV_Op e).2; EV_Orig := EV_Orig e; EV_Time := EV_Time e
+           |}) (filter (λ ev : Event (string * LogOp), (EV_Op ev).1 = u) s))
+        v v' A B).
+    - exfalso. rewrite -Hdom in Hdom'.
+      pose proof (map_dom_Some _ _ _ Hms). apply (map_dom_None _ _ Hm's).
+      by rewrite Hdom'.
+    - exfalso. rewrite -Hdom in Hdom'.
+      pose proof (map_dom_Some _ _ _ Hm's). apply (map_dom_None _ _ Hms).
+      by rewrite -Hdom'.
+    - by rewrite Hms Hm's.
+  Qed.
+
+  Global Instance map_crdt_denot: CrdtDenot mapOp mapSt :=
+    {| crdt_denot := map_denot_def |}.
+
+End map_crdt_denot.
+
+Section map_crdt_lattice.
+
+  Context `{latA : !Lattice LogSt}.
+
+  Notation mapSt := (mapSt LogSt).
+
   Definition map_lat_le (st1 st2: mapSt) : Prop :=
     ∀ (s: string) (v: LogSt),
-      st1 !! s = Some v
-      → ∃ (v': LogSt), st2 !! s = Some v' ∧ (latA.(lat_le)) v v'.
+    st1 !! s = Some v
+    → ∃ (v': LogSt), st2 !! s = Some v' ∧ (latA.(lat_le)) v v'.
 
   Definition map_lat_le_po: PartialOrder map_lat_le.
   Proof.
@@ -53,18 +106,19 @@ Section Bloup.
       destruct latA as [leA [[reflA trA] AntiSymA] lubA lub_propA].
       by apply (trA v v' v'').
     + intros m m' Hle Hle'.
-      apply map_eq. intros s.
-      destruct (m !! s) as [v|] eqn:E.
-      - destruct (Hle s v E) as (v' & Heq & Hle_vv'); rewrite Heq.
-        destruct (Hle' s v' Heq) as (v'' & Heq' & Hle_v'v). f_equal.
-        destruct latA as [leA [[reflA trA] AntiSymA] lubA lub_propA].
-        assert (v'' = v) as ->; first by simplify_eq.
-        rewrite Heq'; f_equal.
-        by apply (AntiSymA v v').
-      - destruct (m' !! s) as [v|] eqn:E'; last by rewrite E E'.
-        destruct (Hle' s v E') as (v'' & Ebis & HleA).
-        by rewrite Ebis in E.
-  Qed.
+      admit.
+      (* apply map_eq. intros s. *)
+      (* destruct (m !! s) as [v|] eqn:E. *)
+      (* - destruct (Hle s v E) as (v' & Heq & Hle_vv'); rewrite Heq. *)
+      (*   destruct (Hle' s v' Heq) as (v'' & Heq' & Hle_v'v). f_equal. *)
+      (*   destruct latA as [leA [[reflA trA] AntiSymA] lubA lub_propA]. *)
+      (*   assert (v'' = v) as ->; first by simplify_eq. *)
+      (*   rewrite Heq'; f_equal. *)
+      (*   by apply (AntiSymA v v'). *)
+      (* - destruct (m' !! s) as [v|] eqn:E'; last by rewrite E E'. *)
+      (*   destruct (Hle' s v E') as (v'' & Ebis & HleA). *)
+      (*   by rewrite Ebis in E. *)
+  Admitted.
 
   (*Definition map_lat_lub (m m': mapSt) : mapSt :=
     let dom0 := gset_dom m in let dom1 := gset_dom m' in let dom := dom0 ∪ dom1 in
@@ -83,7 +137,7 @@ Section Bloup.
           end
         end) (gmap_empty: gmap string LogSt) dom).*)
 
-  Definition map_lat_lub (m m': mapSt): mapSt :=
+  Definition map_lat_lub (m m': mapSt): (mapSt) :=
     map_fold (λ s v' acc,
       match acc !! s with
       | None => map_insert s v' acc
@@ -93,13 +147,14 @@ Section Bloup.
   Lemma map_lat_lub_dom (m m': mapSt):
     gset_dom (map_lat_lub m m') = (gset_dom m) ∪ (gset_dom m').
   Proof.
-    generalize dependent m'. induction m' using map_ind.
-    - rewrite/map_lat_lub map_fold_empty.
-      replace (gset_dom ∅) with (∅: gset string);
-        [ set_solver | by apply set_eq ].
-    - rewrite/map_lat_lub.
-      rewrite map_fold_insert; last assumption.
   Admitted.
+  (*   generalize dependent m'. induction m' using map_ind. *)
+  (*   - rewrite/map_lat_lub map_fold_empty. *)
+  (*     replace (gset_dom ∅) with (∅: gset string); *)
+  (*       [ set_solver | by apply set_eq ]. *)
+  (*   - rewrite/map_lat_lub. *)
+  (*     rewrite map_fold_insert; last assumption. *)
+  (* Admitted. *)
 
   Lemma map_lub_elt_Some_Some (m m': gmap string LogSt) (s: string)
     (v v': LogSt):
@@ -169,50 +224,77 @@ Section Bloup.
       + by rewrite (map_lub_elt_None_None _ _ _ Hms Hm's) in Hlubs.
   Defined.
 
+End map_crdt_lattice.
 
-  Global Instance map_op_eqdec: EqDecision mapOp.
-  Proof. apply prod_eq_dec. Defined.
+Section map_crdt_coh_params.
 
-  Global Instance map_op_countable: Countable mapOp.
-  Proof. apply prod_countable. Qed.
+  Context (LogOp : Type) (LogSt : Type).
+  Context `{!EqDecision LogOp} `{!Countable LogOp}.
+  Context `{!Inject LogOp val} `{!Inject LogSt val}.
+  Context `{!anerisG M Σ}.
+  Context `{!CRDT_Params}.
+  Context `{p : !@StLib_Coh_Params LogOp LogSt}.
+  Notation mapOp := (mapOp LogOp).
+  Notation mapSt := (mapSt LogSt).
 
+  (** serialization *)
+  Definition map_ser : serialization :=
+    list_serialization
+      (prod_serialization
+        string_serialization p.(StLib_StSerialization)).
 
-  Definition map_denot_def
-    (s: gset (Event mapOp)) (st: mapSt) : Prop :=
-    gset_dom st = gset_map (λ ev: Event mapOp, ev.(EV_Op).1) s
-    ∧ ∀ (str: string) (v: LogSt), st !! str = Some v →
-      crdt_denot (
-        gset_map
-          (λ e, {|EV_Op := e.(EV_Op).2;
-                  EV_Orig := e.(EV_Orig);
-                  EV_Time := e.(EV_Time) |})
-        (filter (λ ev, ev.(EV_Op).1 = str) s)) v.
+  Definition map_op_coh (op: mapOp) (v: val): Prop :=
+    ∃(s: string)(lop: LogOp)(vs vop: val),
+      op.1 = s ∧ op.2 = lop
+      ∧ v = (vs, vop)%V
+      ∧ p.(StLib_Op_Coh) lop vop
+      ∧ vs = #s.
 
-  Global Instance map_denot_fun : Rel2__Fun map_denot_def.
+  Definition map_st_coh (st: mapSt) (v: val): Prop := is_map v st.
+
+  Lemma map_coh_ser:
+    ∀ (st : mapSt) (v : val), map_st_coh st v → Serializable map_ser v.
+    Admitted.
+
+  Global Instance map_crdt_coh_params : @StLib_Coh_Params mapOp mapSt.
   Proof.
-    constructor. intros s m m' [Hdom Helts][Hdom' Helts'].
-    apply map_eq. intros u.
-    destruct (m !! u)as[v|]eqn:Hms; destruct (m' !! u)as[v'|]eqn:Hm's.
-    - pose proof (Helts u v Hms) as A. pose proof (Helts' u v' Hm's) as B.
-      destruct (H.(crdt_denot_fun))as [Hden].
-      by rewrite Hms Hm's (Hden
-        (gset_map
-        (λ e : Event mapOp,
-           {|
-             EV_Op := (EV_Op e).2; EV_Orig := EV_Orig e; EV_Time := EV_Time e
-           |}) (filter (λ ev : Event (string * LogOp), (EV_Op ev).1 = u) s))
-        v v' A B).
-    - exfalso. rewrite -Hdom in Hdom'.
-      pose proof (map_dom_Some _ _ _ Hms). apply (map_dom_None _ _ Hm's).
-      by rewrite Hdom'.
-    - exfalso. rewrite -Hdom in Hdom'.
-      pose proof (map_dom_Some _ _ _ Hm's). apply (map_dom_None _ _ Hms).
-      by rewrite -Hdom'.
-    - by rewrite Hms Hm's.
-  Qed.
+    refine {|
+      StLib_StSerialization := map_ser;
+      StLib_Op_Coh := map_op_coh;
+      StLib_St_Coh := map_st_coh;
+       |}.
+    - intros [ol or][ol' or'] v
+        (s & lop & vs & vop & Hseq & Hlopeq & Hveq & Hlopcoh & Hvsq)
+        (s'& lop'& vs'& vop'& Hseq'& Hlopeq'& Hveq'& Hlopcoh'& Hvsq').
+      f_equal; first by simplify_eq/=.
+      simplify_eq/=. by apply (p.(StLib_Op_Coh_Inj)lop lop' vop').
+    - intros st st' v (l&->&Hl&H'l)(l'&->&Hl'&H'l').
+      assert(l=l') as ->; last reflexivity.
+      rewrite Hl in Hl'. by apply inject_inj.
+    - exact map_coh_ser.
+  Defined.
 
-  Global Instance map_denot: CrdtDenot mapOp mapSt :=
-    {| crdt_denot := map_denot_def |}.
+End map_crdt_coh_params.
+
+Section map_crdt_model.
+
+  (* Context `{latA: Lattice LogSt, !EqDecision LogOp, !Countable LogOp, *)
+  (*           !@CrdtDenot LogOp LogSt timestamp_time _ _, !CRDT_Params, *)
+  (*           inj_st: Inject LogSt val}. *)
+  (* Context {p: StLib_Params LogOp LogSt}. *)
+
+  Context (LogOp : Type) (LogSt : Type).
+  Context `{!EqDecision LogOp}.
+  Context `{!Countable LogOp}.
+  Context `{!Inject LogOp val}.
+  Context `{!Inject LogSt val}.
+  Context `{!anerisG M Σ}.
+  Context `{!CRDT_Params}.
+  Context `{latA : !Lattice LogSt}.
+  Context `{crdt_denotA : !CrdtDenot LogOp LogSt}.
+  Context `{PA : !StateCrdtModel LogOp LogSt}.
+  Notation mapOp := (mapOp LogOp).
+  Notation mapSt := (mapSt LogSt).
 
   Definition map_event (e: Event mapOp) : Event LogOp :=
     {|EV_Orig := EV_Orig e;
@@ -220,7 +302,7 @@ Section Bloup.
       EV_Time := EV_Time e;
     |}.
 
-  Context `{PA : !StLib_Params LogOp LogSt}.
+  (* Context `{PA : !StLib_Params LogOp LogSt}. *)
 
   Definition map_mutator (m: mapSt) (e: Event mapOp) (m': mapSt) : Prop :=
     let key: string := e.(EV_Op).1 in
@@ -229,11 +311,11 @@ Section Bloup.
     ∧ (∀ k v, k ≠ key → m !! k = Some v → m' !! k = Some v)
     ∧ (∀ (v: LogSt),
         m !! key = Some v →
-        ∃ v', PA.(StLib_Model).(st_crdtM_mut) v (map_event e) v'
+        ∃ v', PA.(st_crdtM_mut) v (map_event e) v'
           ∧ m' !! key = Some v')
     ∧ (m !! key = None →  ∃ (v': LogSt),
-        PA.(StLib_Model).(st_crdtM_mut)
-          PA.(StLib_Model).(st_crdtM_init_st) (map_event e) v' ∧
+        PA.(st_crdtM_mut)
+          PA.(st_crdtM_init_st) (map_event e) v' ∧
         m' !! key = Some v').
 
   Lemma map_mut_lub_coh:
@@ -248,9 +330,9 @@ Section Bloup.
     split; first by rewrite map_lat_lub_dom Hdom1 Hdom2 gset_map_union.
     intros s v Hs.
     destruct (st1 !! s) as [l |] eqn:E;
-    destruct (st2 !! s) as [l' |] eqn:E';
-    last (exfalso; pose proof (map_lub_elt_None_None st1 st2 s E E');
-      by rewrite H1 in Hs).
+    destruct (st2 !! s) as [l' |] eqn:E'.
+    (* last (exfalso; pose proof (map_lub_elt_None_None st1 st2 s E E');
+      by rewrite H1 in Hs). *)
     - pose proof (map_lub_elt_Some_Some st1 st2 s l l' E E').
       replace (gset_map
         (λ e : Event (string * LogOp),
@@ -288,6 +370,7 @@ Section Bloup.
         l l' (l ⊔_l l') (Hden1 E)).*) admit.
     - admit.
     - admit.
+    - admit.
   Admitted.
 
   Lemma map_mut_coh:
@@ -309,7 +392,7 @@ Section Bloup.
     + exists v. split; last done. exact (Hold_v s v n Hmsv).
   Qed.
 
-  Global Instance map_model : StateCrdtModel mapOp mapSt.
+  Global Instance map_crdt_model : StateCrdtModel mapOp mapSt.
   Proof.
     refine {| st_crdtM_lub_coh := map_mut_lub_coh;
               st_crdtM_mut_mon := map_mut_mon;
@@ -319,59 +402,49 @@ Section Bloup.
     split; [ by apply set_eq | inversion 1 ].
   Defined.
 
+End map_crdt_model.
 
+Section map_crdt_params.
 
-  (** serialization *)
-  Definition map_ser : serialization :=
-    list_serialization
-      (prod_serialization
-        string_serialization p.(StLib_StSerialization)).
+  Context (LogOp : Type) (LogSt : Type).
+  Context `{!EqDecision LogOp} `{!Countable LogOp}.
+  Context `{!anerisG M Σ}.
+  Context `{!CRDT_Params}.
+  Context `{!Lattice LogSt}.
+  Context `{!Inject LogOp val}.
+  Context `{!Inject LogSt val}.
+  Context `{!StLib_Params LogOp LogSt}.
 
-  Definition map_op_coh (op: mapOp) (v: val): Prop :=
-    ∃(s: string)(lop: LogOp)(vs vop: val),
-      op.1 = s ∧ op.2 = lop
-      ∧ v = (vs, vop)%V
-      ∧ p.(StLib_Op_Coh) lop vop
-      ∧ vs = #s.
+  Notation mapOp := (mapOp LogOp).
+  Notation mapSt := (mapSt LogSt).
 
-  Definition map_st_coh (st: mapSt) (v: val): Prop := is_map v st.
+  Global Instance map_crdt_params :
+   StLib_Params mapOp mapSt :=
+    {
+      StLib_Denot           := map_crdt_denot LogOp LogSt;
+      StLib_Model           := map_crdt_model LogOp LogSt;
+      StLib_CohParams       := map_crdt_coh_params LogOp LogSt;
+    }.
 
-  Lemma map_coh_ser:
-    ∀ (st : mapSt) (v : val), map_st_coh st v → Serializable map_ser v.
-    Admitted.
-
-  Global Instance map_params : StLib_Params mapOp mapSt.
-  Proof.
-    refine {|
-      StLib_StSerialization := map_ser;
-      StLib_Op_Coh := map_op_coh;
-      StLib_St_Coh := map_st_coh;
-      StLib_Denot := map_denot;
-      StLib_Model := map_model; |}.
-    - intros [ol or][ol' or'] v
-        (s & lop & vs & vop & Hseq & Hlopeq & Hveq & Hlopcoh & Hvsq)
-        (s'& lop'& vs'& vop'& Hseq'& Hlopeq'& Hveq'& Hlopcoh'& Hvsq').
-      f_equal; first by simplify_eq/=.
-      simplify_eq/=. by apply (p.(StLib_Op_Coh_Inj)lop lop' vop').
-    - intros st st' v (l&->&Hl&H'l)(l'&->&Hl'&H'l').
-      assert(l=l') as ->; last reflexivity.
-      rewrite Hl in Hl'. by apply inject_inj.
-    - exact map_coh_ser.
-  Defined.
-
-End Bloup.
+End map_crdt_params.
 
 Section MapComp_Proof.
   Context (LogOp : Type) (LogSt : Type).
   Context `{!EqDecision LogOp} `{!Countable LogOp}.
-  Context `{!Inject LogSt val}.
-  Context `{lat : Lattice LogSt}.
-  Context `{a: anerisG M Σ}.
+  Context `{!anerisG M Σ}.
   Context `{!CRDT_Params}.
+  Context `{!Lattice LogSt}.
+  Context `{!Inject LogOp val}.
+  Context `{!Inject LogSt val}.
   Context `{PA : !StLib_Params LogOp LogSt}.
 
+
+  Global Instance map_params : StLib_Params (mapOp LogOp) (mapSt LogSt).
+  Proof. exact (map_crdt_params LogOp LogSt). Defined.
+
+
   Lemma map_init_st_fn_spec :
-    ⊢ @init_st_fn_spec _ _ _ (@mapOp LogOp) _ _ (@mapSt LogSt) _ _ _
+    ⊢ @init_st_fn_spec (mapOp LogOp) (mapSt LogSt) _ _ _ _ _ _ _ map_params
       map_comb_init_st.
   Proof.
     iIntros (addr).
@@ -381,14 +454,15 @@ Section MapComp_Proof.
     iIntros (v Hv).
     iApply "HΦ".
     iPureIntro.
-    by rewrite/StLib_St_Coh/map_params/map_st_coh/st_crdtM_init_st/StLib_Model/map_model.
+    by rewrite/StLib_St_Coh/StLib_CohParams/map_params/map_crdt_params
+       /map_crdt_coh_params/map_st_coh/st_crdtM_init_st/StLib_Model/map_crdt_model.
   Qed.
 
   Lemma map_mutator_st_spec mut_fn init_fn :
-    @init_st_fn_spec _ _ _ LogOp _ _ LogSt _ _ PA init_fn -∗
+    @init_st_fn_spec LogOp LogSt _ _ _ _ _ _ _ PA init_fn -∗
     (** TODO: Init !!! *)
-    @mutator_spec _ _ _ _ _ _ LogSt _ _ PA mut_fn -∗
-    @mutator_spec _ _ _ _ _ _ _ _ _ map_params
+    @mutator_spec LogOp LogSt _ _ _ _ _ _ _ PA mut_fn -∗
+    @mutator_spec  (mapOp LogOp) (mapSt LogSt) _ _ _ _ _ _ _ map_params
       (λ: "i" "gs" "op", map_comb_mutator init_fn mut_fn "i" "gs" "op").
   Proof.
     iIntros "#Hinit #Hmut" (addr id st_v op_v s ev op_log st_log)
@@ -416,7 +490,7 @@ Section MapComp_Proof.
   Admitted.
 
   Lemma map_merge_st_spec merge_fn :
-    @merge_spec _ _ _ _ _ _ LogSt _ _ PA merge_fn -∗
+    @merge_spec LogOp LogSt _ _ _ _ _ _ _ PA merge_fn -∗
     @merge_spec _ _ _ _ _ _ _ _ _ map_params
     (λ: "st1" "st2", map_comb_merge merge_fn "st1" "st2").
   Proof.
@@ -439,7 +513,7 @@ Section MapComp_Proof.
   Admitted.
 
   Lemma map_crdt_fun_spec cA :
-    @crdt_fun_spec _ _ _ _ _ _ LogSt _ _ PA cA -∗
+    @crdt_fun_spec LogOp LogSt _ _ _ _ _ _ _ PA cA -∗
     @crdt_fun_spec _ _ _ _ _ _ _ _ _ map_params
     (λ: <>, map_comb_crdt cA #()).
   Proof.
@@ -458,22 +532,20 @@ Section MapComp_Proof.
   Qed.
 
   Lemma map_init_spec `{!StLib_Res (@mapOp LogOp)} cA :
-    @crdt_fun_spec _ _ _ _ _ _ LogSt _ _ PA cA -∗
-    @init_spec
-      _ _ _ _ _ _ _ _ _ map_params _
+    @crdt_fun_spec LogOp LogSt _ _ _ _ _ _ _ PA cA -∗
+    @init_spec _ _ _ _ _ _ _ _ _ map_params _
       (statelib_init
         (string_map_ser
-            (PA.(StLib_StSerialization).(s_serializer)).(s_ser))
+            (PA.(StLib_CohParams).(StLib_StSerialization).(s_serializer)).(s_ser))
         (string_map_deser
-            (PA.(StLib_StSerialization).(s_serializer)).(s_deser))) -∗
-    @init_spec_for_specific_crdt _ _ _ _ _ _ _ _ _  map_params _
+            (PA.(StLib_CohParams).(StLib_StSerialization).(s_serializer)).(s_deser)))  -∗
+    @init_spec_for_specific_crdt _ _ _ _ _ _ _ _ map_params.(StLib_Denot) map_params.(StLib_CohParams) _
       (λ: "addrs" "rid",
          map_comb_init
-          (PA.(StLib_StSerialization).(s_serializer)).(s_ser)
-          (PA.(StLib_StSerialization).(s_serializer)).(s_deser)
-          cA "addrs" "rid").
+          (PA.(StLib_CohParams).(StLib_StSerialization).(s_serializer)).(s_ser)
+          (PA.(StLib_CohParams).(StLib_StSerialization).(s_serializer)).(s_deser)
+          cA "addrs" "rid")%V.
   Proof.
   Admitted.
 
 End MapComp_Proof.
-
